schorr-waite/GraphMark.thy
@@ -5,19 +5,19 @@ begin
 install_C_file "graph_mark.c"
 autocorres [heap_abs_syntax] "graph_mark.c"
 
-definition reach :: "('a \<Rightarrow> 'a set) \<Rightarrow> 'a set \<Rightarrow> 'a set" where
-  "reach f roots = rtrancl { p. snd p \<in> f (fst p) } `` roots"
-
 context graph_mark begin
 
 type_synonym mark = "32 word"
 type_synonym state_pred = "lifted_globals \<Rightarrow> bool"
 
-definition ptr_ok :: "node_C ptr \<Rightarrow> state_pred" where
-  "ptr_ok p s \<equiv> p \<noteq> NULL \<and> is_valid_node_C s p"
-
 definition out :: "lifted_globals \<Rightarrow> node_C ptr \<Rightarrow> node_C ptr set" where
   "out s p \<equiv> { s[p]\<rightarrow>left, s[p]\<rightarrow>right }"
+
+inductive_set reach :: "lifted_globals \<Rightarrow> node_C ptr set \<Rightarrow> node_C ptr set"
+  for s :: lifted_globals and R :: "node_C ptr set"
+  where
+    reach_root: "p \<noteq> NULL \<Longrightarrow> p \<in> R \<Longrightarrow> p \<in> reach s R"
+  | reach_step: "q \<noteq> NULL \<Longrightarrow> q \<in> out s p \<Longrightarrow> p \<in> reach s R \<Longrightarrow> q \<in> reach s R"
 
 definition mark :: "bool \<Rightarrow> node_C \<Rightarrow> node_C" where
   "mark c node \<equiv> if c then node \<lparr> mark_C := 3 \<rparr> else node"
@@ -26,11 +26,8 @@ definition mark_set :: "node_C ptr set \<Rightarrow> lifted_globals \<Rightarrow
   "mark_set R s \<equiv> heap_node_C_update (\<lambda> h p. mark (p \<in> R) (h p)) s"
 
 definition mark_precondition :: "state_pred \<Rightarrow> node_C ptr \<Rightarrow> state_pred" where
-  "mark_precondition P root \<equiv> \<lambda> s. let R = reach (out s) {root} in
-    (\<forall> p \<in> R. ptr_ok p s \<and> s[p]\<rightarrow>mark = 0) \<and> P (mark_set R s)"
-
-primrec roots :: "node_C ptr \<times> node_C ptr \<Rightarrow> node_C ptr set" where
-  "roots (p,q) = { r \<in> {p,q}. r \<noteq> NULL }"
+  "mark_precondition P root \<equiv> \<lambda> s. let R = reach s {root} in
+    (\<forall> p \<in> R. is_valid_node_C s p \<and> s[p]\<rightarrow>mark = 0) \<and> P (mark_set R s)"
 
 type_synonym path_upd_t =
   "lifted_globals \<Rightarrow> node_C ptr set
@@ -47,7 +44,7 @@ primrec tail_upd :: path_upd_t where
     else None)"
 
 primrec path_upd :: path_upd_t where
-  "path_upd s M r q p [] = (if p = NULL \<and> q = r \<and> r \<in> M then Some s else None)" |
+  "path_upd s M r q p [] = (if p = NULL \<and> q = r \<and> (r = NULL \<or> r \<in> M) then Some s else None)" |
   "path_upd s M r q p (p' # ps) =
    (if p \<noteq> p' then None
     else if s[p]\<rightarrow>mark = 0 then
@@ -62,24 +59,23 @@ primrec mark_invariant :: "state_pred \<Rightarrow> node_C ptr \<Rightarrow> nod
   "mark_invariant P root (p,q) s =
     (\<exists> t u path M.
       let
-        R = reach (out t) {root};
+        R = reach t {root};
         U = R - M;
         F = U - set path
       in
-        root \<noteq> NULL \<and>
         P t \<and>
         set path \<subseteq> R \<and>
         M \<subseteq> R \<and>
-        reach (out s) (roots (p,q)) = R \<and>
-        reach (out t) M = M \<and>
+        reach s {p,q} = R \<and>
+        reach t M = M \<and>
         path_upd s M root q p path = Some u \<and>
         mark_set U u = t \<and>
-        (\<forall> p \<in> R. ptr_ok p s) \<and>
+        (\<forall> p \<in> R. is_valid_node_C s p) \<and>
         (\<forall> p \<in> M. s[p]\<rightarrow>mark = 3) \<and>
         (\<forall> p \<in> F. s[p]\<rightarrow>mark = 0))"
 
-primrec mark_measure :: "(node_C ptr \<times> node_C ptr) \<times> lifted_globals \<Rightarrow> nat" where
-  "mark_measure (r,s) = setsum (\<lambda> p. 3 - unat s[p]\<rightarrow>mark) (reach (out s) (roots r))"
+fun mark_measure :: "(node_C ptr \<times> node_C ptr) \<times> lifted_globals \<Rightarrow> nat" where
+  "mark_measure ((p,q),s) = setsum (\<lambda> p. 3 - unat s[p]\<rightarrow>mark) (reach s {p,q})"
 
 definition mark_incr :: "node_C ptr \<Rightarrow> lifted_globals \<Rightarrow> lifted_globals" where
   "mark_incr p \<equiv> heap_node_C_update (\<lambda> h. h(p := mark_C_update (\<lambda> m. m + 1) (h p)))"
@@ -94,7 +90,7 @@ lemma mark_incr_right [simp]: "(mark_incr q s)[p]\<rightarrow>right = s[p]\<righ
   unfolding mark_incr_def by (simp add: fun_upd_def graph_mark.get_node_right_def)
 
 lemma out_mark_incr [simp]: "out (mark_incr q s) = out s"
-  unfolding out_def[abs_def] by auto
+  unfolding out_def[abs_def] by fastforce
 
 lemma mark_set_left [simp]: "(mark_set R s)[p]\<rightarrow>left = s[p]\<rightarrow>left"
   unfolding mark_set_def mark_def by (simp add: graph_mark.get_node_left_def)
@@ -103,7 +99,7 @@ lemma mark_set_right [simp]: "(mark_set R s)[p]\<rightarrow>right = s[p]\<righta
   unfolding mark_set_def mark_def by (simp add: graph_mark.get_node_right_def)
 
 lemma out_mark_set [simp]: "out (mark_set R s) = out s"
-  unfolding out_def[abs_def] by auto
+  unfolding out_def[abs_def] by fastforce
 
 lemma mark_incr_node_valid [simp]: "is_valid_node_C (mark_incr q s) p = is_valid_node_C s p"
   unfolding mark_incr_def by simp
@@ -118,31 +114,35 @@ lemma mark_incr_right_upd [simp]:"(mark_incr q s)[p\<rightarrow>right := v] = ma
   by (smt fun_upd_def fun_upd_twist fun_upd_upd graph_mark.update_node_right_def
           lifted_globals.surjective lifted_globals.update_convs(5) node_C_updupd_diff(1))
 
-lemma roots_simp [simp]:
-  "root \<noteq> NULL \<Longrightarrow> {r. (r = NULL \<or> r = root) \<and> r \<noteq> NULL} = {root}"
-  by blast
-
-lemma null_path_empty:
+lemma null_path_empty [dest]:
   assumes
     "path_upd s M root q NULL path = Some u"
-    "set path \<subseteq> R"
-    "\<forall> p \<in> R. ptr_ok p s"
+    "set path \<subseteq> reach t roots"
   shows
     "path = []"
-  using assms by (cases path, auto simp: ptr_ok_def)
+  using assms by (cases path; auto elim: reach.cases)
+
+lemma reachable_subset: assumes "R \<subseteq> S" shows "reach s R \<subseteq> reach s S"
+  proof -
+    { fix p have "p \<in> reach s R \<Longrightarrow> R \<subseteq> S \<Longrightarrow> p \<in> reach s S"
+      by (induction rule: reach.induct) (auto intro: reach.intros) }
+    thus ?thesis using assms by auto
+  qed
+
+lemma reachable_with_null: "reach s R = S \<Longrightarrow> R' = insert NULL R \<Longrightarrow> reach s R' = S"
+  sorry
+
+lemma reachable_null [simp]: "reach s {NULL} = {}"
+  proof -
+    { fix p have "p \<in> reach s {NULL} \<Longrightarrow> False" by (induction rule: reach.induct) auto }
+    thus ?thesis by auto
+  qed
+
+lemma reachable_empty [simp]: "reach s {} = {}"
+  by (metis empty_subsetI graph_mark.reachable_subset reachable_null subset_antisym)
 
 lemma mark_set_empty [simp]: "mark_set {} u = u"
   unfolding mark_set_def mark_def by simp
-
-lemma reach_root:
-  assumes
-    "reach f M = M"
-    "root \<in> M"
-  shows
-    "reach f {root} - M = {}"
-  using assms
-  unfolding reach_def
-  sorry
 
 lemma graph_mark'_correct: "\<lbrace> mark_precondition P root \<rbrace> graph_mark' root \<lbrace> \<lambda> _. P \<rbrace>!"
   unfolding
@@ -154,17 +154,18 @@ lemma graph_mark'_correct: "\<lbrace> mark_precondition P root \<rbrace> graph_m
    sorry
   subgoal for q s t u path M
    apply (clarsimp simp: Let_def)
-   apply (frule (2) null_path_empty)
+   apply (frule (1) null_path_empty)
    apply (clarsimp split: split_if_asm)
-   apply (frule (1) reach_root)
+   apply (cases "root = NULL"; clarsimp)
+   apply (frule reachable_subset[of "{root}" M t, simplified])
    by auto
   subgoal for s
-   apply (rule exI[where x="mark_set (reach (out s) {root}) s"])
+   apply (rule exI[where x="mark_set (reach s {root}) s"])
    apply (rule exI[where x=s])
-   apply (rule exI[where x="[root]"])
+   apply (rule exI[where x="if root = NULL then [] else [root]"])
    apply (rule exI[where x="{}"])
-   apply (simp add: Let_def)
-   by (auto simp: reach_def ptr_ok_def)
+   apply (cases "root = NULL"; clarsimp simp: Let_def)
+   sorry
   done
 
 end
